persistent typing judgment, empty env for functions

theories/logrel_heaplang_sessions/ltyping.v
@@ -6,7 +6,7 @@ From iris.heap_lang Require Import notation proofmode.
 (* The semantic typing judgment *)
 Definition ltyped `{heapG Σ}
     (Γ : gmap string (lty Σ)) (e : expr) (A : lty Σ) : iProp Σ :=
-  (∀ vs, env_ltyped Γ vs -∗ WP subst_map vs e {{ A }})%I.
+  (□ ∀ vs, env_ltyped Γ vs -∗ WP subst_map vs e {{ A }})%I.
 
 Notation "Γ ⊨ e : A" := (ltyped Γ e A)
   (at level 100, e at next level, A at level 200).
