theories/logrel_heaplang_sessions/split.v
@@ -8,12 +8,12 @@ Section EnvironmentSplitting.
   Implicit Types A : lty Σ.
 
   (* TODO: Should this be an iProp or just a Prop? Is it ever the case that splitting an environment is only allowed when you have some resource? *)
-  Definition env_split Γ Γ1 Γ2 : iProp Σ := (∀ vs, env_ltyped Γ vs -∗ env_ltyped Γ1 vs ∗ env_ltyped Γ2 vs)%I.
+  Definition env_split Γ Γ1 Γ2 : iProp Σ := (□ ∀ vs, env_ltyped Γ vs -∗ env_ltyped Γ1 vs ∗ env_ltyped Γ2 vs)%I.
 
   Lemma env_split_empty:
     env_split ∅ ∅ ∅.
   Proof.
-    iIntros (vs) "H".
+    iIntros (vs) "!> H".
     iSplitL; by rewrite /env_ltyped big_sepM_empty.
   Qed.
 
@@ -21,7 +21,7 @@ Section EnvironmentSplitting.
     Γ !! x = None → env_split Γ Γ1 Γ2 -∗ env_split (<[x := A]> Γ) (<[x := A]> Γ1) Γ2.
   Proof.
     intros HΓx.
-    iIntros "Hsplit" (vs) "HΓ".
+    iIntros "#Hsplit" (vs) "!> HΓ".
     iPoseProof (big_sepM_insert with "HΓ") as "[Hv HΓ]"; try assumption.
     iPoseProof ("Hsplit" with "HΓ") as "[HΓ1 HΓ2]". iFrame.
     iApply (big_sepM_insert_2 with "[Hv]"); simpl; iFrame.
@@ -30,7 +30,7 @@ Section EnvironmentSplitting.
   Lemma env_split_comm Γ Γ1 Γ2:
     env_split Γ Γ1 Γ2 -∗ env_split Γ Γ2 Γ1.
   Proof.
-    iIntros "Hsplit" (vs) "HΓ".
+    iIntros "#Hsplit" (vs) "!> HΓ".
     iDestruct ("Hsplit" with "HΓ") as "[HΓ1 HΓ2]".
     iFrame.
   Qed.
@@ -39,7 +39,7 @@ Section EnvironmentSplitting.
     Γ !! x = None → env_split Γ Γ1 Γ2 -∗ env_split (<[x := A]> Γ) Γ1 (<[x := A]> Γ2).
   Proof.
     intros HΓx.
-    iIntros "Hsplit".
+    iIntros "#Hsplit".
     iApply env_split_comm.
     iApply env_split_left; try assumption.
       by iApply env_split_comm.
@@ -49,12 +49,13 @@ Section EnvironmentSplitting.
   Lemma env_split_copy Γ Γ1 Γ2 (x : string) A:
     Γ !! x = None → LTyCopy A → env_split Γ Γ1 Γ2 -∗ env_split (<[x := A]> Γ) (<[x := A]> Γ1) (<[x := A]> Γ2).
   Proof.
-    intros Hcopy HΓx. iIntros "Hsplit" (vs) "HΓ".
+    intros Hcopy HΓx. iIntros "#Hsplit" (vs) "!> HΓ".
     iPoseProof (big_sepM_insert with "HΓ") as "[Hv HΓ]"; try assumption.
     iDestruct "Hv" as (v ?) "#HAv".
     iPoseProof ("Hsplit" with "HΓ") as "[HΓ1 HΓ2]".
     iSplitL "HΓ1"; iApply big_sepM_insert_2; simpl; iFrame; eauto.
   Qed.
 
-  Definition env_copy Γ Γ' : iProp Σ := (∀ vs, env_ltyped Γ vs -∗ □ env_ltyped Γ' vs)%I.
+  (* TODO: Should this be a Prop, just like env_split perhaps? *)
+  Definition env_copy Γ Γ' : iProp Σ := (□ (∀ vs, env_ltyped Γ vs -∗ □ env_ltyped Γ' vs))%I.
 End EnvironmentSplitting.
