theories/logrel_heaplang_sessions/rules/prod.v
@@ -21,7 +21,7 @@ Section properties.
   Lemma ltyped_pair Γ Γ1 Γ2 e1 e2 A1 A2 :
     env_split Γ Γ1 Γ2 -∗ (Γ1 ⊨ e1 : A1) -∗ (Γ2 ⊨ e2 : A2) -∗ Γ ⊨ (e1,e2) : A1 * A2.
   Proof.
-    iIntros "Hsplit H1 H2" (vs) "HΓ /=".
+    iIntros "#Hsplit #H1 #H2" (vs) "!> HΓ /=".
     iPoseProof ("Hsplit" with "HΓ") as "[HΓ1 HΓ2]".
     wp_apply (wp_wand with "(H2 [HΓ2 //])"); iIntros (w2) "HA2".
     wp_apply (wp_wand with "(H1 [HΓ1 //])"); iIntros (w1) "HA1".
@@ -32,10 +32,10 @@ Section properties.
   doesn't work because the result has to be of the type A * (any * B),
   which is useless since it is a pair again. *)
   Definition split : val := λ: "pair" "f", "f" (Fst "pair") (Snd "pair").
-  Lemma ltyped_split Γ A1 A2 B:
-    Γ ⊨ split : (A1 * A2 → (A1 → A2 → B) → B)%lty.
+  Lemma ltyped_split A1 A2 B:
+    ∅ ⊨ split : (A1 * A2 → (A1 → A2 → B) → B)%lty.
   Proof.
-    iIntros (vs) "HΓ /=".
+    iIntros (vs) "!> HΓ /=".
     wp_apply wp_value.
     iIntros (v) "Hv".
     iDestruct "Hv" as (w1 w2 ->) "[Hw1 Hw2]".
