theories/logrel_heaplang_sessions/rules/ref.v
@@ -22,9 +22,10 @@ Section properties.
   Proof. iIntros (v). by iDestruct 1 as (i w ->) "?". Qed.
 
   Definition refalloc : val := λ: "init", ref "init".
-  Lemma ltyped_alloc Γ A : Γ ⊨ refalloc : (A → ref A)%lty.
+  Lemma ltyped_alloc A :
+    ∅ ⊨ refalloc : (A → ref A)%lty.
   Proof.
-    iIntros (vs) "HΓ /=".
+    iIntros (vs) "!> HΓ /=".
     wp_apply wp_value.
     iIntros (v) "Hv". rewrite /refalloc. wp_pures.
     wp_alloc l as "Hl".
@@ -38,9 +39,10 @@ Section properties.
   unmodified, but moves the resources, in the sense that you can no
   longer use the memory at the old location. *)
   Definition refload : val := λ: "r", (!"r", "r").
-  Lemma ltyped_load Γ A : Γ ⊨ refload : (ref A → A * ref any)%lty.
+  Lemma ltyped_load A :
+    ∅ ⊨ refload : (ref A → A * ref any)%lty.
   Proof.
-    iIntros (vs) "HΓ /=".
+    iIntros (vs) "!> HΓ /=".
     wp_apply wp_value.
     iIntros (v) "Hv".
     iDestruct "Hv" as (l w ->) "[Hl Hw]".
@@ -54,10 +56,10 @@ Section properties.
   Qed.
 
   Definition refstore : val := λ: "r" "new", "r" <- "new";; "r".
-  Lemma ltyped_store Γ A B:
-    Γ ⊨ refstore : (ref A → B → ref B)%lty.
+  Lemma ltyped_store A B:
+    ∅ ⊨ refstore : (ref A → B → ref B)%lty.
   Proof.
-    iIntros (vs) "HΓ /=".
+    iIntros (vs) "!> HΓ /=".
     wp_apply wp_value.
     iIntros (v) "Hv".
     iDestruct "Hv" as (l old ->) "[Hl Hold]".
